p256_adx in CLI, not particularly clean

src/Arithmetic/WeightStream.v
@@ -12,45 +12,6 @@ Require Import Crypto.Util.ZUtil.Tactics.PullPush.Modulo.
 Require Import Crypto.Util.ZUtil.Tactics.RewriteModSmall.
 Import ListNotations. Local Open Scope list_scope. Local Open Scope Z_scope.
 
-(*
-Goal forall W s c a b, 0 <= c -> W < s ->
-  0 <= a < s ->
-  0 <= c*b <= W-c ->
-  s <= (a + c*b) ->
-  (((a + c*b) mod s) / W = ((a + c*b) mod s + c * ((a + c*b) / s)) / W).
-Proof.
-  intros; assert ((a + c * b) / s = 1) by (Z.div_mod_to_equations; nia).
-  transitivity 0; Z.div_mod_to_equations; nia.
-Qed.
-
-Goal forall W s (HH: s / W * W = s) c a b, 0 <= c < W -> W < s ->
-  0 <= a < s ->
-  0 <= -c*b < W-c ->
-  (a + c*b) < 0 ->
-  (((a + c*b) mod s) / W = ((a + c*b) mod s + c * ((a + c*b) / s)) / W).
-Proof.
-  intros; assert ((a + c * b) / s = -1) by (Z.div_mod_to_equations; nia).
-  assert ((a + c * b) mod s = s + a + c*b) by (Z.div_mod_to_equations; nia).
-  rewrite H4 in *; rewrite H5 in *.
-  enough ((s + a + c * b) / W - (s/W-1) = (s + a + c * b + c * -1) / W - (s/W-1)) by lia.
-  rewrite <-2Z.div_sub with (b:=s/W-1) by lia; rewrite 2Z.div_small; trivial.
-  all : rewrite ?HH; try split; ring_simplify; try nia.
-Qed.
- *)
-
-Lemma saturated_pseudomersenne_reduction_converges :
-  forall W s c a b (HH: b < 0 -> s / W * W = s), 0 <= c < W -> W <= s ->
-  0 <= a < s ->
-  0 <= c*Z.abs b <= W-c ->
-  (((a + c*b) mod s) / W = ((a + c*b) mod s + c * ((a + c*b) / s)) / W).
-Proof.
-  intros; assert ((a+c*b)/s = -1 \/ (a+c*b)/s = 0 \/ (a+c*b)/s = 1)
-    by (Z.div_mod_to_equations; nia); intuition idtac.
-  { clear -HH H H0 H2 H4 H7. transitivity (s/W-1); Z.div_mod_to_equations; nia. }
-  { f_equal. rewrite Z.mod_small; Z.div_mod_to_equations; lia. }
-  { clear -H0 H3 H4 H6 H7. transitivity 0; Z.div_mod_to_equations; nia. }
-Qed.
-
 Require Import Crypto.Language.PreExtra.
 
 Module Pos.
@@ -142,7 +103,7 @@ Module stream.
   Proof. cbv [tl prefixes map]. rewrite firstn_S; trivial. Qed.
 End stream. Notation stream := stream.stream.
 
-Module Saturated. Section __.
+Module Saturated.
   Import List ListNotations.
   Import stream Coq.Init.Datatypes Coq.Lists.List List.
 
@@ -198,7 +159,7 @@ Module Saturated. Section __.
 
   Import Morphisms.
 
-  Instance Proper_eval : Proper (pointwise_relation _ eq==>eq==>eq)%signature eval.
+  Global Instance Proper_eval : Proper (pointwise_relation _ eq==>eq==>eq)%signature eval.
   Proof.
     cbv [pointwise_relation].
     intros f g fg l; revert fg; revert g; revert f; induction l; intros;
@@ -244,7 +205,7 @@ Module Saturated. Section __.
     x mod (stream.hd bound) :: encode (stream.tl bound) n (x / stream.hd bound).
   Proof. trivial. Qed.
 
-  Instance Proper_encode : Proper (pointwise_relation _ eq ==> eq ==> eq ==> eq)%signature encode.
+  Global Instance Proper_encode : Proper (pointwise_relation _ eq ==> eq ==> eq ==> eq)%signature encode.
   Proof.
     intros f f' F n; revert F; revert f'; revert f; induction n;
       repeat intro; subst; rewrite ?encode_O, ?encode_S; trivial.
@@ -469,9 +430,25 @@ Module Saturated. Section __.
   Definition product_scan_ bound acc pps h c o :=
     let '(l, h) := product_scan bound acc pps h c o in
     dlet r := l ++ if Z.of_nat (length pps) <? Z.of_nat (length acc)
-                   then add_ bound 0 (skipn (length pps) acc) [h]
+                   then add_ (stream.skipn (length l) bound) 0 (skipn (length pps) acc) [h]
                    else [h] in
     r.
+
+  Lemma eval_product_scan_ bound acc pps h c o :
+    eval bound (product_scan_ bound acc pps h c o)
+    = eval bound acc + h + c + o + eval bound (map (uncurry Z.mul) pps).
+  Proof.
+    cbv [product_scan_ Let_In].
+    rewrite product_scan_correct, eval_app, eval_encode, length_encode.
+    case (Z.ltb_spec (Z.of_nat (length pps)) (Z.of_nat (length acc))) as [H|H]; cycle 1;
+      repeat rewrite ?eval_cons, ?eval_nil, ?Z.mul_0_r, ?eval_add_, ?Z.add_0_l, ?Z.add_0_r.
+    { rewrite <-!Z.add_assoc, <-Z.add_mod_idemp_l, eval_firstn, Z.add_mod_idemp_l, !Z.add_assoc by lia.
+      rewrite ?firstn_all2 by lia. Z.div_mod_to_equations; nia. }
+    pose proof firstn_skipn (length pps) acc as Hacc.
+    eapply (f_equal (eval bound)) in Hacc; erewrite eval_app in Hacc.
+    rewrite firstn_length, Nat.min_l in * by lia.
+    Z.div_mod_to_equations; nia.
+  Qed.
 
   Definition add_mul_small bound acc x ys : list Z * Z :=
     let '(lo, (h, c, o)) := product_scan' bound acc (map (pair x) ys) 0 0 0 in
@@ -568,135 +545,6 @@ Module Saturated. Section __.
   Lemma length_mul bound xs ys : ys <> [] ->  length (mul bound xs ys) = (length xs + length ys)%nat.
   Admitted.
 
-
-  (* See lemma saturated_pseudomersenne_reduction_converges *)
-  Definition reduce' bound k (c : Z) (a : list Z) (b : list Z) : list Z :=
-    let (sum, carry) := add_mul_small bound a c b in
-    let (sum', _) := add bound 0 sum [c * carry] in
-    firstn k sum' ++ skipn k sum.
-
-  Lemma eval_reduce' bound k c a b m
-    (s : Z := weight bound (Nat.max (length a) (length b))) (Hc : s mod m = c)
-    (Hc' : 0 <= c < weight bound k) (Hla : (k <= length a)%nat)
-    (Ha : 0 <= eval bound a < weight bound (length a))
-    (Hb : c * Z.abs (eval bound b) <= weight bound k - c) :
-    eval bound (reduce' bound k c a b) mod m = (eval bound a + s * eval bound b) mod m.
-  Proof.
-    cbv [reduce'] in *.
-    repeat (rewrite ?add_mul_small_correct, ?add_correct, ?firstn_encode, ?eval_app,
-      ?eval_encode, ?length_encode, ?eval_skipn_encode, ?eval_cons, ?eval_nil,
-      ?Z.add_0_l, ?Z.mul_0_r, ?Z.add_0_r by lia; cbn [fst snd length]); fold s.
-    rewrite saturated_pseudomersenne_reduction_converges, <-Z.div_mod''; try split; try lia.
-    { rewrite (Zmod_eq _ s) by lia. push_Zmod. rewrite ?Hc. pull_Zmod. f_equal. ring. }
-    { intros. rewrite Z.mul_comm. symmetry; apply Z.div_exact; try apply mod_weight_le; lia. }
-    { apply weight_mono_le; lia. }
-    { enough (weight bound (length a) <= s) by lia. apply weight_mono_le. lia. }
-  Qed.
-
-  Definition reduce bound k (c : Z) (a : list Z) (b : list Z) : list Z :=
-    (* NOTE: it would be nice if we had an "if" that threw error messages during specialization *)
-    if ((Z.of_nat k <=? Z.of_nat (length a))
-    && (Z.of_nat (length b) <=? Z.of_nat (length a))
-    && (0 <=? c)
-    && (c <? weight bound k)
-    && (0 <=? eval bound a)
-    && (eval bound a <? weight bound (length a))
-    && (c*Z.abs (eval bound b) <=? weight bound k - c))%bool
-    then reduce' bound k c a b
-    else a ++ b.
-
-  Lemma eval_reduce bound k c a b m
-    (s : Z := weight bound (length a)) (Hc : s mod m = c)
-    (Hbound : pointwise_relation nat eq (stream.skipn (length a) bound) bound) :
-    eval bound (reduce bound k c a b) mod m = (eval bound a + s * eval bound b) mod m.
-  Proof.
-    cbv [reduce]; break_match.
-    { repeat match goal with H : _ |- _ => apply Bool.andb_prop in H; case H as [H ?] end.
-      Require Import Crypto.Util.Decidable.Bool2Prop.
-      rewrite eval_reduce'; rewrite ?Nat.max_l; repeat split; auto; try apply Nat2Z.inj_le; auto. }
-    { rewrite eval_app; subst s. f_equiv. f_equiv. f_equiv. f_equiv. trivial. }
-  Qed.
-
-  (*
-  Definition mul_short_mod bound c n (a b : list Z) :=
-    let p := mul bound a b in
-    let (lo, hi) := (firstn n p, skipn n p) in
-    if (* true by range analysis *) c*Z.abs (eval bound hi) <=? weight bound (length hi) - c
-    then reduce' bound (length hi) c  lo hi
-    else p.
-  *)
-
-  Definition mulmod bound n c a b :=
-    dlet p := mul bound a b in
-    let (lo, hi) := add_mul_limb bound (firstn n p) c (skipn n p) in
-    if (* true by range analysis *) c*Z.abs hi <=? weight bound 1 - c
-    then reduce' bound 1 c lo [hi]
-    else lo ++ [hi].
-
-  Lemma eval_mulmod B (bound := fun _ => B) n a b m
-    (s : Z := weight bound n) (c := s mod m) (Hc' : 0 <= c < stream.hd bound)
-    (Hn : (n <= length a + length b <= n + n)%nat) (Hb : b <> nil)
-    : eval bound (mulmod bound n c a b) mod m = (eval bound a * eval bound b) mod m.
-  Proof.
-    cbv [Let_In mulmod].
-    assert (1 <= length b)%nat by (destruct b; cbn [length] in *; congruence || lia).
-    pose proof (eq_refl : weight bound n mod m = c) as Hc.
-    pose proof eval_mul B a b as Hmul; fold bound in Hmul.
-    epose proof eq_sym (eval_app _ (firstn n _) (skipn n _)) as Hsplit.
-    erewrite firstn_skipn, Hmul in Hsplit.
-    replace (length (firstn n (mul bound a b))) with n in *
-      by (rewrite firstn_length, length_mul; trivial; lia).
-    apply (f_equal (fun x => x mod m)) in Hsplit.
-    revert Hsplit; push_Zmod; rewrite ?Hc; pull_Zmod; intro.
-    change (stream.skipn n bound) with bound in *.
-    rewrite add_mul_limb_correct.
-    set (t := eval bound (firstn n (mul bound a b)) +
-      c * eval bound (skipn n (mul bound a b))) in *.
-    progress replace (Nat.max (length (firstn n (mul bound a b))) (length (skipn n (mul bound a b))))
-      with n in * by (rewrite firstn_length, skipn_length, !length_mul; trivial; lia).
-    break_match; [rewrite eval_reduce', eval_encode, Z.add_comm | rewrite eval_app];
-    repeat rewrite ?length_encode, ?firstn_length, ?skipn_length, ?length_mul, ?eval_cons,
-                   ?eval_encode, ?eval_nil, ?Z.mul_0_r, ?Z.add_0_r, ?weight_1 in *;
-    cbn [length]; replace (Nat.max n 1) with n by lia; trivial; try lia.
-    { rewrite <-Z.div_mod by lia. rewrite Hsplit; trivial. }
-    { apply Z.mod_pos_bound. lia. }
-    rewrite Z.add_comm. rewrite <-Z.div_mod; lia.
-  Qed.
-
-  Definition addmod bound c a b :=
-    let (sum, carry) := add bound 0 a b in
-    reduce' bound 1 c sum [carry].
-
-  Lemma eval_addmod bound c a b m
-    (s : Z := weight bound (length a)) (Hc : s mod m = c)
-    (Hc' : 0 <= 2*c <= bound O)
-    (Hla : (1 < length a)%nat) (Hlb : (length b <= length a)%nat)
-    (Ha : 0 <= eval bound a < weight bound (length a))
-    (Hb : - weight bound (length a) <= eval bound b <= weight bound (length a)) :
-    eval bound (addmod bound c a b) mod m = (eval bound a + eval bound b) mod m.
-  Proof.
-    cbv [addmod]; rewrite add_correct by trivial; rewrite ?Z.add_0_l.
-    rewrite eval_reduce'; rewrite ?eval_encode, ?length_encode, ?weight_1,
-    ?eval_cons, ?eval_nil; cbn [length]; rewrite ?Nat.max_l, ?Z.mul_0_r, ?Z.add_0_r by lia; 
-      try solve [trivial | cbn; lia | apply Z.mod_pos_bound; lia ].
-    { rewrite (Z.add_comm (_ mod _) (_ * (_ / _))), <-Z.div_mod; lia. }
-    assert (Z.abs ((eval bound a + eval bound b) / Z.pos (weight bound (length a))) <= 1) by (Z.div_mod_to_equations; nia); nia.
-  Qed.
-
-  Lemma eval_map_opp bound xs : eval bound (map Z.opp xs) = - eval bound xs.
-  Proof. revert bound; induction xs; trivial; intros; rewrite ?map_cons, ?eval_cons, ?IHxs; lia. Qed.
-
-  Definition submod bound c a b := addmod bound c a (map Z.opp b).
-
-  Lemma eval_submod bound c a b m
-    (s : Z := weight bound (length a)) (Hc : s mod m = c)
-    (Hc' : 0 <= 2*c <= bound O)
-    (Hla : (1 < length a)%nat) (Hlb : (length b <= length a)%nat)
-    (Ha : 0 <= eval bound a < weight bound (length a))
-    (Hb : - weight bound (length a) <= eval bound b <= weight bound (length a)) :
-    eval bound (submod bound c a b) mod m = (eval bound a - eval bound b) mod m.
-  Proof. cbv [submod]; rewrite eval_addmod; rewrite ?map_length, ?eval_map_opp; auto; lia. Qed.
-
   Definition select c a b := map (uncurry (Z.zselect c)) (combine a b).
 
   Lemma select_correct c a b : length a = length b -> select c a b = if dec (c = 0) then a else b.
@@ -711,6 +559,9 @@ Module Saturated. Section __.
   Proof. cbv [cswap]; intros; rewrite !select_correct; break_match; congruence. Qed.
 
   Definition condsub bound a b := let (lo, hi) := add bound 0 a (map Z.opp b) in select (-hi) lo a.
+
+  Lemma eval_map_opp bound xs : eval bound (map Z.opp xs) = - eval bound xs.
+  Proof. revert bound; induction xs; trivial; intros; rewrite ?map_cons, ?eval_cons, ?IHxs; lia. Qed.
 
   Lemma condsub_correct bound a b :
     0 <= eval bound a < weight bound (length a) ->
@@ -801,39 +652,4 @@ Module Saturated. Section __.
       rewrite Z.rem_mul_r by nia.
       rewrite Z.mod_add', Z.mod_mod by lia; trivial. }
   Qed.
-
-
-  Local Notation "!" := ltac:(vm_decide) (only parsing).
-  Goal forall a0 a1 a2 a3 b : Z, False. intros.
-  Proof.
-    pose proof (eval_reduce' (fun _ => 2^64)%positive 1 38 [a0;a1;a2;a3] [b] (2^256-38) ! ! !).
-    cbn [length] in *.
-    change ((weight (fun _ : nat => (2 ^ 64)%positive) 4%nat)) with (2^256)%positive in *.
-    change ((weight (fun _ : nat => (2 ^ 64)%positive) 1%nat)) with (2^64)%positive in *.
-    change (weight (fun _ : nat => (2 ^ 64)%positive) 1%nat)%positive with (2^64)%positive in *.
-    set (eval (fun _ : nat => (2 ^ 64)%positive)) as eval in *.
-    set (reduce' (fun _ : nat => (2 ^ 64)%positive) _ _ _) as reduce' in *.
-  Abort.
-
-  Goal forall a0 a1 a2 a3 b0 b1 b2 b3 : Z, False. intros.
-  Proof.
-    pose proof (eval_addmod (fun _ => 2^64)%positive 38 [a0;a1;a2;a3] [b0;b1;b2;b3] (2^256-38) ! ! ! !).
-    cbn [length] in *.
-    change ((weight (fun _ : nat => (2 ^ 64)%positive) 4%nat)) with (2^256)%positive in *.
-    change ((weight (fun _ : nat => (2 ^ 64)%positive) 1%nat)) with (2^64)%positive in *.
-    change (weight (fun _ : nat => (2 ^ 64)%positive) 1%nat)%positive with (2^64)%positive in *.
-    set (eval (fun _ : nat => (2 ^ 64)%positive)) as eval in *.
-    set (addmod _ _) as addmod in *.
-  Abort.
-
-  Goal forall a0 a1 a2 a3 b0 b1 b2 b3 : Z, False. intros.
-  Proof.
-    pose proof (eval_mulmod (2^64)%positive 4 [a0;a1;a2;a3] [b0;b1;b2;b3] (2^256-38) ! ! !).
-    cbn [length] in *.
-    change ((weight (fun _ : nat => (2 ^ 64)%positive) 4%nat)) with (2^256)%positive in *.
-    set (eval (fun _ : nat => (2 ^ 64)%positive)) as eval in *.
-    change (2 ^ 256 mod (2 ^ 256 - 38)) with 38 in *.
-    set (mulmod _ _) as mulmod in *.
-  Abort.
-End __.
 End Saturated.
