src/PushButtonSynthesis/P256ADXReificationCache.v
@@ -1,0 +1,58 @@
+Require Import Coq.ZArith.ZArith.
+Require Import Coq.derive.Derive.
+Require Import Crypto.Arithmetic.P256ADX. Import WeightStream Saturated.
+Require Import Crypto.PushButtonSynthesis.ReificationCache.
+Local Open Scope Z_scope.
+
+Import
+  Language.API.Compilers
+  Language.Wf.Compilers.
+Local Set Keyed Unification. (* needed for making [autorewrite] fast, c.f. COQBUG(https://github.com/coq/coq/issues/9283) *)
+
+Derive reified_p256_mul
+       SuchThat (is_reification_of reified_p256_mul p256_mul)
+       As reified_p256_mul_correct.
+Proof. 
+  Time
+  instantiate (1:=
+    (ltac:(
+      let e := constr:(p256_mul) in
+      let e := eval cbv delta [two_steps_of_p256_montgomery_reduction p256_mul mul add_mul add_mul_limb_ add_mul_limb product_scan product_scan_ stream.map weight stream.prefixes] in e in
+      let r := Reify e in
+      exact r))
+    ) in (value of reified_p256_mul).
+  split. { intros. exact eq_refl. }
+  { prove_Wf ltac:(()). }
+Time Qed.
+
+Derive reified_p256_sqr
+       SuchThat (is_reification_of reified_p256_sqr p256_sqr)
+       As reified_p256_sqr_correct.
+Proof. 
+  Time
+  instantiate (1:=
+    (ltac:(
+      let e := constr:(p256_sqr) in
+      let e := eval cbv delta [p256_sqr sqr4 two_steps_of_p256_montgomery_reduction p256_mul mul add_mul add_mul_limb_ add_mul_limb product_scan product_scan_ stream.map weight stream.prefixes] in e in
+      let r := Reify e in
+      exact r))
+    ) in (value of reified_p256_sqr).
+  split. { intros. exact eq_refl. }
+  { prove_Wf ltac:(()). }
+Time Qed.
+
+#[global]
+ Hint Extern 1 (_ = _) => apply_cached_reification p256_mul (proj1 reified_p256_mul) : reify_cache_gen.
+#[global]
+ Hint Immediate (proj2 reified_p256_mul_correct) : wf_gen_cache.
+#[global]
+ Hint Rewrite (proj1 reified_p256_mul_correct) : interp_gen_cache.
+Local Opaque reified_p256_mul. (* needed for making [autorewrite] not take a very long time *)
+
+#[global]
+ Hint Extern 1 (_ = _) => apply_cached_reification p256_sqr (proj1 reified_p256_sqr) : reify_cache_gen.
+#[global]
+ Hint Immediate (proj2 reified_p256_sqr_correct) : wf_gen_cache.
+#[global]
+ Hint Rewrite (proj1 reified_p256_sqr_correct) : interp_gen_cache.
+Local Opaque reified_p256_sqr. (* needed for making [autorewrite] not take a very long time *)
