src/PushButtonSynthesis/SaturatedPseudoMersenneReificationCache.v
@@ -1,14 +1,4 @@
-(** * Push-Button Synthesis of Solinas Reduction: Reification Cache *)
-Require Import Coq.QArith.QArith_base Coq.QArith.Qround.
-Require Import Coq.Init.Nat.
-Require Import Coq.ZArith.ZArith.
-Require Import Coq.ZArith.BinInt.
-Require Import Coq.derive.Derive.
-Require Import Crypto.Arithmetic.Core.
-Require Import Crypto.Arithmetic.ModOps.
-Require Import Crypto.Arithmetic.Saturated.
-Require Import Crypto.Arithmetic.SolinasReduction.
-Require Import Crypto.PushButtonSynthesis.ReificationCache.
+(** * Push-Button Synthesis of Saturated pseude-Mersenne reduction: Reification Cache *)
 
 Require Import Crypto.Language.IdentifierParameters.
 Require Import Coq.Strings.String.
@@ -18,6 +8,18 @@ Require Import Crypto.Util.ZRange.
 Require Import Crypto.Util.ZUtil.Definitions.
 Require Import Crypto.Language.PreExtra.
 
+Require Import Coq.Init.Nat.
+Require Import Coq.ZArith.ZArith.
+Require Import Coq.ZArith.BinInt.
+Require Import Coq.derive.Derive.
+Require Import Crypto.Arithmetic.Core.
+Require Import Crypto.Arithmetic.ModOps.
+Require Import Crypto.Arithmetic.Saturated.
+Require Import Crypto.Arithmetic.SaturatedPseudoMersenne.
+Require Import Crypto.PushButtonSynthesis.ReificationCache.
+
+Import WeightStream WeightStream.Saturated.
+
 Local Open Scope Z_scope.
 
 Local Set Keyed Unification. (* needed for making [autorewrite] fast, c.f. COQBUG(https://github.com/coq/coq/issues/9283) *)
@@ -25,24 +27,43 @@ Local Set Keyed Unification. (* needed for making [autorewrite] fast, c.f. COQBU
 Import
   Language.API.Compilers
   Language.Wf.Compilers.
-Import SolinasReduction.SolinasReduction.
 
 Module Export SolinasReduction.
 
   Derive reified_add_gen
-         SuchThat (is_reification_of reified_add_gen add)
+         SuchThat (is_reification_of reified_add_gen addmod)
          As reified_add_gen_correct.
   Proof. Time cache_reify (). Time Qed.
 
   Derive reified_mul_gen
          SuchThat (is_reification_of reified_mul_gen mulmod)
          As reified_mul_gen_correct.
-  Proof. Time cache_reify (). Time Qed.
+  Proof. 
+    Time
+    instantiate (1:=(ltac:(
+        let e := constr:(mulmod) in
+        let e := eval cbv delta [mulmod mul add_mul add_mul_limb_ add_mul_limb reduce' product_scan stream.map weight stream.prefixes] in e in
+        let r := Reify e in
+        exact r)))
+      in (value of reified_mul_gen).
+    split. { intros. exact eq_refl. }
+    { prove_Wf ltac:(()). }
+  Time Qed.
 
   Derive reified_square_gen
-         SuchThat (is_reification_of reified_square_gen squaremod)
+         SuchThat (is_reification_of reified_square_gen (fun bound n z a => mulmod bound n z a a))
          As reified_square_gen_correct.
-  Proof. Time cache_reify (). Time Qed.
+  Proof. 
+    Time
+    instantiate (1:=(ltac:(
+        let e := constr:((fun bound n z a => mulmod bound n z a a)) in
+        let e := eval cbv delta [mulmod mul add_mul add_mul_limb_ add_mul_limb reduce' product_scan stream.map weight stream.prefixes] in e in
+        let r := Reify e in
+        exact r)))
+      in (value of reified_square_gen).
+    split. { intros. exact eq_refl. }
+    { prove_Wf ltac:(()). }
+  Time Qed.
 
   #[global]
    Hint Extern 1 (_ = _) => apply_cached_reification addmod (proj1 reified_add_gen) : reify_cache_gen.
@@ -61,7 +82,7 @@ Module Export SolinasReduction.
   Local Opaque reified_mul_gen. (* needed for making [autorewrite] not take a very long time *)
 
   #[global]
-   Hint Extern 1 (_ = _) => apply_cached_reification squaremod (proj1 reified_square_gen) : reify_cache_gen.
+   Hint Extern 1 (_ = _) => apply_cached_reification Positional.squaremod (proj1 reified_square_gen) : reify_cache_gen.
   #[global]
    Hint Immediate (proj2 reified_square_gen_correct) : wf_gen_cache.
   #[global]
